code/ecdsa/Hacl.Impl.EC.PointAddMixed.fsti
@@ -23,8 +23,9 @@ val point_add_mixed: #c: curve -> p: point c -> q: pointAffine c -> result: poin
     live h p /\ live h q /\ live h result /\ live h tempBuffer /\ 
     eq_or_disjoint q result /\ disjoint p q /\ disjoint p tempBuffer /\ 
     disjoint q tempBuffer /\ disjoint p result /\ disjoint result tempBuffer /\  
-    point_eval c h p /\ 
-      (let x, y = getXAff q, getYAff q in 
-      felem_eval c h x /\ felem_eval c h y))
-  (ensures fun h0 _ h1 -> modifies (loc tempBuffer |+| loc result) h0 h1 /\ point_eval c h1 result /\
-    fromDomainPoint #c #DH (point_as_nat c h1 result) == _point_add_mixed #c (fromDomainPoint #c #DH (point_as_nat c h0 p)) (fromDomainPointAffine #c (point_affine_as_nat c h0 q)))
+    point_eval c h p /\ point_aff_eval c h q)
+  (ensures fun h0 _ h1 -> modifies (loc tempBuffer |+| loc result) h0 h1 /\ point_eval c h1 result /\ (
+    let qX, qY, qZ = point_affine_x_as_nat c h0 q, point_affine_y_as_nat c h0 q, 1 in 
+    let qD = fromDomainPoint #c #DH (qX, qY, qZ) in 
+    fromDomainPoint #c #DH (point_as_nat c h1 result) == 
+    _point_add_mixed #c (fromDomainPoint #c #DH (point_as_nat c h0 p)) qD))
